Election by elbow-grease

examples/Election.v
@@ -10,8 +10,8 @@ From CTree Require Import
   CTree.Logic.State
   CTree.Logic.Iter
   CTree.Logic.Bind
-  CTree.Events.Writer
-  CTree.Events.Net.Uniring.
+  CTree.Interp.State
+  CTree.Events.Writer.
 
 From Coq Require Import
   Fin
@@ -19,90 +19,207 @@ From Coq Require Import
   List
   Classes.SetoidClass.
 
+From ExtLib Require Import
+  Data.Monads.StateMonad.
+
 Set Implicit Arguments.
 
-Import ListNotations CTreeNotations CtlNotations.
-Local Close Scope list_scope.
+Import CtlNotations CTreeNotations.
 Local Open Scope ctree_scope.
 Local Open Scope fin_vector_scope.
 Local Open Scope ctl_scope.
 
 Section Election.
   Context {n: nat}.
-  Variant message :=
-    | Candidate (u: fin' n)
-    | Elected (u: fin' n).
-
-  Notation netE := (netE message).
-
-  Definition msg_id(m: message): fin' n :=
-    match m with
-    | Candidate u => u
-    | Elected u => u
-    end.
-
-  Definition eqb_message(a b: message): bool :=
-    match a, b with
-    | Candidate a, Candidate b => Fin.eqb a b
-    | Elected a, Elected b => Fin.eqb a b
-    | _, _ => false
-    end.
-
-  Notation continue := (Ret (inl tt)).
-  Notation stop := (Ret (inr tt)).
+  Notation Id := (fin' n).
   
+  (*| Message passing in unidirectional ring |*)
+  Variant msg :=
+    | Candidate (u: Id)
+    | Elected   (u: Id).
+
+  Variant netE: Type :=
+    | Recv
+    | Send (m: msg)
+    | Seti (id: Id)
+    | Geti.
+  
+  Global Instance encode_netE: Encode netE :=
+    fun e => match e with
+          | Recv => msg
+          | Send _ => unit
+          | Seti _ => unit
+          | Geti => Id
+          end.
+  
+  Definition send: msg -> ctree netE unit :=
+    fun p => Ctree.trigger (Send p).
+  
+  Definition recv: ctree netE msg :=
+    Ctree.trigger Recv.
+
+  Definition set: Id -> ctree netE unit :=
+    fun id => Ctree.trigger (Seti id).
+
+  Definition get: ctree netE Id :=
+    Ctree.trigger Geti. 
+    
+  Notation Mails := (vec' n msg).
+  Notation NetObs := (Id * msg).
+  
+  (* Spinlock instrumented semantics: (counter, lock state, shared state) *)
+  Definition h_netE(cycle: fin' n -> fin' n): netE ~> stateT (Id * Mails) (ctreeW NetObs) := 
+    fun e =>
+      mkStateT
+        (fun '(id, mail) =>
+           match e return ctreeW NetObs (encode e * (fin' n * vec' n msg)) with
+           | Send msg =>
+               log (id, msg) ;;
+               Ret (tt, (id, mail @ cycle id := msg))
+           | Recv =>
+               log (id, mail $ id) ;;
+               Ret (mail $ id, (id, mail))
+           | Geti =>
+               Ret (id, (id, mail))
+           | Seti id =>
+               Ret (tt, (id, mail))
+           end).
+    
   (* Always terminates, conditional on receiving either:
      1. (Candidate candidate), where candidate = id -- I received my own [id] back 
      2. (Elected leader) -- Someone else was elected [leader]
    *)
   Definition elect(id: fin' n): ctree netE unit :=
-    send (Candidate id) ;;
-    (* Recv loop *)
-    Ctree.iter
+    m <- recv ;;
+    match m with
+    | Candidate candidate =>
+        match Fin_compare candidate id with (* candidate < id *)
+        (* [left] neighbor proposed candidate, support her to [right]. *)
+        | Gt => send (Candidate candidate)
+        (* [left] neighbor proposed a candidate, do not support her. *)
+        | Lt => Ret tt
+        (* I am the leader, but only I know. Tell my [right] and return. *)
+        | Eq => send (Elected id)
+        end
+    | Elected leader =>
+        (* I am a follower and know the [leader] *)
+        send (Elected leader)
+    end.
+
+  (* Uniring scheduler, picks initial [i] nondeterministically, then runs forever *)
+  Definition elect_sched(cycle: fin' n -> fin' n): ctree netE void :=
+    i <- Ctree.branch n ;;
+    set i ;;
+    Ctree.forever void
       (fun _ =>
-         m <- recv ;;
-         match m with
-         | Some (Candidate candidate) =>
-             match Fin_compare candidate id with (* candidate < id *)
-             (* [left] neighbor proposed candidate, support her to [right]. *)
-             | Gt => send (Candidate candidate) ;; continue
-             (* [left] neighbor proposed a candidate, do not support her. *)
-             | Lt => continue
-             (* I am the leader, but only I know. Tell my [right] and return. *)
-             | Eq => send (Elected id) ;; stop
-             end
-         | Some (Elected leader) =>
-             (* I am a follower and know the [leader] *)
-             send (Elected leader) ;; stop
-         | None =>  stop (* Recv loop *)
-         end) tt.
+         i <- get ;;
+         elect i ;;
+         set (cycle i)
+      ) tt.
 
-  Definition election_proto : ctree (writerE NetObs) void :=
-    uring_sched (Vector.map (fun id => {| mbox := None; proc := elect id |}) (fin_all_v n)).
+End Election.
 
-  Lemma election_fair: forall (i: fin' n),
-      <( election_proto, Pure |= AF visW {fun obs => obs.(id) = i} )>.
-  Proof with auto with ctl.
-    intros.
-    unfold election_proto, uring_sched. 
-    unfold Ctree.branch.
-    rewrite bind_br.
-    cright.
-    apply axl_br; split; [csplit; split; auto with ctl|].
-    intro c. (* Nondeterministic pick *)
-    rewrite bind_ret_l.
-    unfold Ctree.forever.    
-    eapply aul_iter.
-      with (f:=fun 'tt l _ => List.length l)
-           (Ri:=fun 'tt l w => not_done w /\
-                  match w with
-                  | Obs (Log s') tt =>
-                      match l with
-                      | nil => nl = s'
-                      | h :: ts => exists hs, h :: ts = hs ++ [nl]
-                      end
-                  | _ => exists hs, l = hs ++ [nl]
-                  end)... 
-    intros [] l w (Hd & Hw).
+From Equations Require Import Equations.
+(* Run election for 3 workers *)
+Import Fin.
+Import VectorNotations.
+Open Scope vector_scope.
+
+Equations cycle(i: fin' 2) : fin' 2 :=
+  cycle Fin.F1 := Fin.FS Fin.F1;
+  cycle (Fin.FS Fin.F1) := Fin.FS (Fin.FS Fin.F1);
+  cycle (Fin.FS (Fin.FS Fin.F1)) := Fin.F1.
+
+(* Initial mailboxes are [F3, F1, F2] *)
+Definition mailboxes: vec' 2 (fin' 2) := 
+  Vector.cons _ (FS (FS F1)) _ (Vector.cons _ F1 _ (Vector.cons _ (FS F1) _ (Vector.nil _))).
+
+Import Vectors.
+Local Typeclasses Transparent equ.
+Local Typeclasses Transparent sbisim.
+
+Lemma election3_liveness:
+  <( {interp_state
+        (h_netE cycle)
+        (elect_sched cycle) (F1, Vector.map Candidate mailboxes)}, Pure |=
+          AF visW {fun '(id, msg) => exists e, msg = Elected e /\ id = e /\ e = FS (FS F1)} )>.
+Proof with auto with ctl.
+  intros.
+  unfold elect_sched, Ctree.forever.  
+  cbn.
+  rewrite interp_state_bind.
+  unfold Ctree.branch.
+  rewrite interp_state_br, bind_br.
+  apply aul_br; right; split.
+  - csplit...
+  - intros i.
+    rewrite sb_guard, interp_state_ret, bind_ret_l, interp_state_bind.
+    setoid_rewrite (@interp_state_trigger _ _ _ _ _ _ (Seti _) _); cbn.
+    rewrite bind_bind, bind_ret_l, bind_guard, sb_guard, bind_ret_l.
+    rewrite interp_state_unfold_iter, interp_state_map, bind_map.
+    rewrite interp_state_bind, bind_bind.
+    setoid_rewrite (@interp_state_trigger _ _ _ _ _ _ Geti _); cbn.
+    rewrite bind_bind, bind_ret_l, sb_guard, bind_ret_, interp_state_bind, bind_bind.
+    (* Get into [elect] *)
+    unfold elect.
+    rewrite interp_state_bind, bind_bind. 
+    rewrite (@interp_state_trigger _ _ _ _ _ _ Recv _); cbn.             
+    repeat setoid_rewrite bind_bind.
+    eapply aul_log_r...
+    rewrite bind_ret_, sb_guard, bind_ret_l.
+    ddestruction i; [|ddestruction i]; simpl; simp cycle.
+    + (* Start with F1 *)
+      setoid_rewrite (@interp_state_trigger _ _ _ _ _ _ (Send (Candidate _)) _); simpl.   
+      repeat setoid_rewrite bind_bind.
+      apply aul_log_r...
+      rewrite bind_ret_l, sb_guard, bind_ret_l.
+      setoid_rewrite (@interp_state_trigger _ _ _ _ _ _ (Seti _) _); simpl.
+      setoid_rewrite bind_bind.
+      rewrite bind_ret_l, sb_guard, bind_ret_l, sb_guard.
+      simp cycle; cbn.
+      (* F2 *)
+      unfold iter, MonadIter_ctree.
+      rewrite interp_state_unfold_iter, interp_state_map, bind_map.
+      rewrite interp_state_bind, bind_bind. 
+      rewrite (@interp_state_trigger _ _ _ _ _ _ Geti _); cbn.             
+      rewrite bind_bind, bind_ret_l, sb_guard, bind_ret_l, interp_state_bind, bind_bind,
+        interp_state_bind, bind_bind.
+      setoid_rewrite (@interp_state_trigger _ _ _ _ _ _ Recv _); cbn.
+      repeat setoid_rewrite bind_bind.
+      apply aul_log_r...
+      rewrite bind_ret_l, sb_guard, bind_ret_l; cbn.
+      setoid_rewrite (@interp_state_trigger _ _ _ _ _ _ (Send _) _); simpl.
+      repeat setoid_rewrite bind_bind.
+      eapply aul_log_r...
+      rewrite bind_ret_l, sb_guard, bind_ret_l.
+      setoid_rewrite (@interp_state_trigger _ _ _ _ _ _ (Seti _) _); simpl.
+      setoid_rewrite bind_bind.
+      rewrite bind_ret_l, sb_guard, bind_ret_l, sb_guard.
+      simp cycle; cbn.
+      (* F3 *)
+      unfold iter, MonadIter_ctree.
+      rewrite interp_state_unfold_iter, interp_state_map, bind_map.
+      rewrite interp_state_bind, bind_bind. 
+      rewrite (@interp_state_trigger _ _ _ _ _ _ Geti _); cbn.             
+      rewrite bind_bind, bind_ret_l, sb_guard, bind_ret_l, interp_state_bind, bind_bind,
+        interp_state_bind, bind_bind.
+      setoid_rewrite (@interp_state_trigger _ _ _ _ _ _ Recv _); cbn.
+      repeat setoid_rewrite bind_bind.
+      apply aul_log_r...
+      rewrite bind_ret_l, sb_guard, bind_ret_l; cbn.
+      setoid_rewrite (@interp_state_trigger _ _ _ _ _ _ (Send _) _); simpl.
+      repeat setoid_rewrite bind_bind.
+      eapply aul_log_r...
+      rewrite bind_ret_l, sb_guard, bind_ret_l.
+      setoid_rewrite (@interp_state_trigger _ _ _ _ _ _ (Seti _) _); simpl.
+      setoid_rewrite bind_bind.
+      rewrite bind_ret_l, sb_guard, bind_ret_l, sb_guard.
+      simp cycle; cbn.
+      (* Done *)
+      cleft.
+      csplit.
+      eexists; intuition.
+    + (* F2 *)
+
   Admitted.    
 End Election.
